Mixed.v
@@ -1,6 +1,7 @@
 From Coq Require Import
      List
      Lia
+     Relations
      Arith.Arith.
 
 From ExtLib Require Import
@@ -13,6 +14,8 @@ From ExtLib Require Import
 
 Import ListNotations.
 
+Set Implicit Arguments.
+
 Module Mixed.
   Variable uid : Set.
   Variable var : Set.
@@ -23,73 +26,51 @@ Module Mixed.
   Global Existing Instance eqdec_var.
   Global Existing Instance eqdec_uid.
 
-  (** Time is represented as a nat *)
-  Definition time := nat.
-  
-  (** State is a history of heaps *)
-  Definition heap := var -> nat.
-  Definition history := uid -> time -> heap.
-
-  (** Assume a map from uid * time * var -> nat that acts as a finite map *)
-  Parameter history_map: Map (uid * time * var) nat history.
-  Global Existing Instance history_map.
-
-  #[refine]
-  Global Instance key_reldec: RelDec (@eq (uid * time * var)) := {}.
-  intros [[u1 t1] v1] [[u2 t2] v2].
-  exact (andb (andb (rel_dec u1 u2) (t1 =? t2)) (rel_dec v1 v2)).
-  Defined.
-
   Inductive loop_outcome(acc: Type) :=
   | Done (a : acc)
   | Again (a : acc).
 
-  (** cmd [list of teachers] [list of students] T *)
-  Inductive cmd : list uid -> list uid -> Type -> Type :=
-  | Return {A: Set} (r : A) : cmd [] [] A
-  | Bind {A B} {i1 i2 o1 o2} (c1 : cmd i1 o1 A)
-         (c2 : A -> cmd i2 o2 B): cmd (i1 ++ i2) (o1 ++ o2) B
-  | Recv {i o} (a : var)(from: uid): cmd (from :: i) o var
-  | Send {i o} {A: Set} (r: A) (to: uid) : cmd i (to::o) unit
-  | Loop {i o} {acc : Set} (init : acc)
-         (body : acc -> cmd i o (loop_outcome acc)) : cmd i o acc.
+  (** cmd *)
+  Inductive cmd : Type -> Type :=
+  | Return {A: Set} (r : A) : cmd A
+  | Bind {A B} (c1 : cmd A)
+         (c2 : A -> cmd B): cmd B
+  | Recv (a : var)(from: uid): cmd var
+  | Send {A: Set} (r: A) (to: uid) : cmd unit
+  | Loop {acc : Set} (init : acc)
+         (body : acc -> cmd (loop_outcome acc)) : cmd acc.
  
   Notation "x <- c1 ; c2" := (Bind c1 (fun x => c2)) (right associativity, at level 80).
-  Notation "'for' x := i 'loop' c1 'done'" := (Loop i (fun x => c1)) (right associativity, at level 80).
+  Notation "'for' x := i 'loop' c1 'done'" :=
+    (Loop i (fun x => c1)) (right associativity, at level 80).
 
-  Inductive step : forall {A i o}, uid * time * history * cmd i o A -> heap * cmd A -> Prop :=
-  | StepBindRecur : forall result result'
+  (** No state for now, except my own uid *)
+  Definition local := uid.
+                
+  (** LTS *)
+  Inductive lstep : forall A, local * cmd A -> local * cmd A -> Prop :=
+  | StepBindRecur : forall result result' l l'
                       (c1 c1' : cmd result')
-                      (c2 : result' -> cmd result) h h',
-      step (h, c1) (h', c1')
-      -> step (h, Bind c1 c2) (h', Bind c1' c2)
+                      (c2 : result' -> cmd result),
+      lstep (l, c1) (l', c1') ->
+      lstep (l, Bind c1 c2) (l', Bind c1' c2)
   | StepBindProceed : forall (result result' : Set)
-                        (v : result')
-                        (c2 : result' -> cmd result) h,
-    step (h, Bind (Return v) c2) (h, c2 v)
-  | StepLoop : forall (acc : Set) (init : acc) (body : acc -> cmd (loop_outcome acc)) h,
-    step (h, Loop init body) (h, o <- body init; match o with
-                                                 | Done a => Return a
-                                                 | Again a => Loop a body
-                                                 end).
+                        (v : result') l
+                        (c2 : result' -> cmd result),
+    lstep (l, Bind (Return v) c2) (l, c2 v)
+  | StepLoop : forall (acc : Set) (init : acc) l
+                      (body : acc -> cmd (loop_outcome acc)),
+      lstep (l, Loop init body) (l, o <- body init; match o with
+                                                   | Done a => Return a
+                                                   | Again a => Loop a body
+                                                   end).
 
-  | StepRead : forall h a v,
-    h $? a = Some v
-    -> step (h, Read a) (h, Return v)
-  | StepWrite : forall h a v v',
-    h $? a = Some v
-    -> step (h, Write a v') (h $+ (a, v'), Return tt).
+  Inductive blocked: forall A, cmd A -> Prop :=
+  | RecvBlock: forall a u, blocked (Recv a u)
+  | SendBlock: forall {A: Set} {a: A} u, blocked (Send a u).
+
+  Inductive returned: forall A, cmd A -> Prop :=
+  | DoneCmd: forall {A: Set} {n: A}, returned (Return n).
 
 
-  Definition trsys_of (h : heap) {result} (c : cmd result) := {|
-    Initial := {(h, c)};
-    Step := step (A := result)
-  |}.
-
-  Definition multistep_trsys_of (h : heap) {result} (c : cmd result) := {|
-    Initial := {(h, c)};
-    Step := (step (A := result))^*
-                                                                       |}.
-
-Notation "x <- c1 ; c2" := (Bind c1 (fun x => c2)) (right associativity, at level 80).
-Infix "||" := Par.
+End Mixed.
